Fixed bugs in Merkle tree impl.

secure_api/merkle_tree/MerkleTree.New.Low.fst
@@ -292,7 +292,7 @@ let create_mt init =
   create_mt_ hs 32ul;
   V.assign hs 0ul (RV.insert_copy hcpy (V.index hs 0ul) init);
   let rhs = RV.create hreg 32ul in
-  B.malloc HH.root (MT 0ul 1ul hs true rhs) 1ul
+  B.malloc HH.root (MT 0ul 1ul hs false rhs) 1ul
 
 /// Destruction (free)
 
@@ -351,24 +351,19 @@ val construct_rhs:
   hs:hash_vv{V.size_of hs = 32ul} ->
   rhs:hash_vec{V.size_of rhs = 32ul} ->
   j:uint32_t ->
-  acc:hash -> actd:bool ->
+  acc:hash ->
   HST.ST unit
 	 (requires (fun h0 -> true))
 	 (ensures (fun h0 _ h1 -> true))
-let rec construct_rhs lv hs rhs j acc actd =
+let rec construct_rhs lv hs rhs j acc =
   admit ();
   if j = 0ul then ()
-  else if j % 2ul = 0ul
-  then
-    // If `j` is even, it already has a rightmost hash of (lv + 1ul)
-    construct_rhs (lv + 1ul) hs rhs (j / 2ul) acc actd
-  else (
-    (if actd
-    then (hash_2 (V.index (V.index hs lv) (j - 1ul)) acc acc;
-	 RV.assign_copy hcpy rhs (lv + 1ul) acc)
-    else (let copy = Cpy?.copy hcpy in
-	 copy (V.index (V.index hs lv) (j - 1ul)) acc));
-    construct_rhs (lv + 1ul) hs rhs (j / 2ul) acc true)
+  else 
+    (if j % 2ul = 0ul
+    then ()
+    else (RV.assign_copy hcpy rhs lv acc;
+	 hash_2 (V.index (V.index hs lv) (j - 1ul)) acc acc);
+    construct_rhs (lv + 1ul) hs rhs (j / 2ul) acc)
 
 // Construct a Merkle path for a given index `k`, hashes `hs`, 
 // and rightmost hashes `rhs`.
@@ -386,33 +381,38 @@ val mt_get_path_:
 let rec mt_get_path_ lv hs rhs j k path =
   admit ();
   if j <= 1ul then ()
-  else 
-    (if k % 2ul = 0ul
-    then (if k = j then ()
-	 else if k + 1ul < j
-	 then B.upd path 0ul (V.insert (B.index path 0ul)
-				       (V.index (V.index hs lv) (k + 1ul)))
-	 else B.upd path 0ul (V.insert (B.index path 0ul) (V.index rhs lv)))
-    else B.upd path 0ul (V.insert (B.index path 0ul) 
-				  (V.index (V.index hs lv) (k - 1ul)));
-    mt_get_path_ (lv + 1ul) hs rhs (j / 2ul) (k / 2ul) path)
+  else
+    (if k % 2ul = 1ul
+    then B.upd path 0ul (V.insert (B.index path 0ul)
+				  (V.index (V.index hs lv) (k - 1ul)))
+    else
+      (if k + 1ul = j then ()
+      else if k + 2ul = j 
+      then B.upd path 0ul (V.insert (B.index path 0ul) (V.index rhs lv))
+      else B.upd path 0ul (V.insert (B.index path 0ul)
+  	 			    (V.index (V.index hs lv) (k + 1ul))));
+    mt_get_path_ (lv + 1ul) hs rhs ((j + 1ul) / 2ul) (k / 2ul) path)
 
 val mt_get_path:
   mt:mt_p -> 
   idx:uint32_t -> // {MT?.i mt <= idx && idx < MT?.j mt}
-  root:hash ->
+  ih:hash ->
   path:B.pointer (V.vector hash) ->
+  root:hash ->
   HST.ST uint32_t
 	 (requires (fun h0 -> true))
 	 (ensures (fun h0 _ h1 -> true))
-let mt_get_path mt idx root path =
+let mt_get_path mt idx ih path root =
   admit ();
+  let copy = Cpy?.copy hcpy in
   let mtv = B.index mt 0ul in
   if not (MT?.rhs_ok mtv) then
-    (construct_rhs 0ul (MT?.hs mtv) (MT?.rhs mtv) (MT?.j mtv) root false;
+    (copy (V.index (V.index (MT?.hs mtv) 0ul) (MT?.j mtv - 1ul)) root;
+    construct_rhs 0ul (MT?.hs mtv) (MT?.rhs mtv) (MT?.j mtv - 1ul) root;
     B.upd mt 0ul (MT (MT?.i mtv) (MT?.j mtv) (MT?.hs mtv) true (MT?.rhs mtv)))
   else ();
   mt_get_path_ 0ul (MT?.hs mtv) (MT?.rhs mtv) (MT?.j mtv) idx path;
+  copy (V.index (V.index (MT?.hs mtv) 0ul) idx) ih;
   MT?.j mtv
 
 /// Flushing
@@ -453,11 +453,12 @@ let rec mt_verify_ k j path ppos acc =
   admit ();
   if j <= 1ul then ()
   else (if k % 2ul = 0ul
-       then (if k = j then mt_verify_ (k / 2ul) (j / 2ul) path ppos acc
+       then (if k + 1ul = j 
+	    then mt_verify_ (k / 2ul) ((j + 1ul) / 2ul) path ppos acc
 	    else (hash_2 acc (V.index path ppos) acc;
-		 mt_verify_ (k / 2ul) (j / 2ul) path (ppos + 1ul) acc))
+		 mt_verify_ (k / 2ul) ((j + 1ul) / 2ul) path (ppos + 1ul) acc))
        else (hash_2 (V.index path ppos) acc acc;
-	    mt_verify_ (k / 2ul) (j / 2ul) path (ppos + 1ul) acc))
+	    mt_verify_ (k / 2ul) ((j + 1ul) / 2ul) path (ppos + 1ul) acc))
 
 val buf_eq:
   #a:eqtype -> b1:B.buffer a -> b2:B.buffer a ->
@@ -477,14 +478,14 @@ let rec buf_eq #a b1 b2 len =
 val mt_verify:
   k:uint32_t ->
   j:uint32_t{k < j} ->
+  ih:hash ->
   path:V.vector hash{V.size_of path > 0ul} ->
   root:hash ->
   HST.ST bool
 	 (requires (fun h0 -> true))
 	 (ensures (fun h0 _ h1 -> true))
-let mt_verify k j path root =
+let mt_verify k j ih path root =
   admit ();
-  let acc = B.malloc HH.root 0uy hash_size in
-  mt_verify_ k j path 0ul acc;
-  buf_eq acc root hash_size
+  mt_verify_ k j path 0ul ih;
+  buf_eq ih root hash_size
 
